\begin{equation}
h^f() = h^f_{ref} -(T-T_{ref})c_p^f \approx 0 - 4.186*  C^\circ   
\end{equation}
where \(h_{ref}^f=0\) and \(T_{ref} = 273.16\, K^\circ\) so that temperature is now measured in centigrades. Assume also \(C^\circ >0 \).
At the same time for \(g\) is 
\begin{equation}
h^g( ) \approx 2.26  - 1.996 C^\circ
\end{equation}
and therefore:
\begin{equation}
h^g()-h^f() \approx 2.26 - 2.19 C^\circ \, {\rm if}\ C^\circ > 0
\end{equation}
For what regards \( c_p\), we have:
\begin{equation}
c_p() = c_p^e \theta^e + 4.186 \theta^
\end{equation}